proof: port subst mappings

Capless/Subst/Basic.lean
@@ -409,6 +409,15 @@ def CVarSubst.ext {Γ : Context n m k}
       rw [<- SType.weaken_crename]
       constructor
       assumption
+  case cmap_bound =>
+    intro c B hb
+    have ⟨b0, hb', he0⟩ := Context.var_cbound_inv hb
+    cases b0 <;> cases he0
+    have h := σ.cmap_bound _ _ hb'
+    rw [<- CBound.crename_rename_comm]
+    rw [<- CaptureSet.weaken_csingleton]
+    rw [<- CBound.weaken_upper]
+    apply Subbound.weaken; easy
 
 def CVarSubst.text {Γ : Context n m k}
   (σ : CVarSubst Γ f Δ) :
@@ -440,6 +449,12 @@ def CVarSubst.text {Γ : Context n m k}
         have hb'' := σ.cmap _ _ hb'
         constructor
         trivial
+    case cmap_bound =>
+      intro c b hb
+      cases hb
+      rename_i hb0
+      have h0 := σ.cmap_bound _ _ hb0
+      apply Subbound.tweaken; easy
     case lmap =>
       intros l S hb
       cases hb
@@ -507,6 +522,27 @@ def CVarSubst.cext {Γ : Context n m k}
       rw [<- SType.cweaken_crename]
       constructor
       assumption
+  case cmap_bound =>
+    intros c b0 hb
+    have hb' := Context.cvar_cbound_inv hb
+    cases hb'
+    case inl h =>
+      have ⟨he1, he2⟩ := h
+      subst he1
+      cases b <;> cases he2
+      simp [FinFun.ext_zero]
+      rename_i cb
+      cases cb
+      case star =>
+        simp [CBinding.crename, CBound.crename]
+        constructor
+      case upper D0 =>
+        constructor
+        apply Subcapt.cbound
+        rw [<- CaptureSet.cweaken_def]
+        rw [<- CaptureSet.cweaken_crename]
+        constructor
+    case inr h => sorry
 
 def VarSubst.open
   (hx : Typed Γ (Term.var x) (EType.type T) Cx) :
@@ -693,7 +729,7 @@ def TVarSubst.open :
 
 def CVarSubst.open :
   CVarSubst
-    (Γ.cvar CBinding.bound)
+    (Γ.cvar (CBinding.bound (CBound.upper {c=c})))
     (FinFun.open c)
     Γ := by
   constructor
@@ -718,6 +754,8 @@ def CVarSubst.open :
     simp [FinFun.open_comp_weaken]
     simp [CaptureSet.crename_id]
     trivial
+  case cmap_bound =>
+    sorry
   case lmap =>
     intro l S hb
     cases hb
@@ -727,7 +765,7 @@ def CVarSubst.open :
 
 def CVarSubst.instantiate {Γ : Context n m k} :
   CVarSubst
-    (Γ.cvar CBinding.bound)
+    (Γ.cvar (CBinding.bound CBound.star))
     FinFun.id
     (Γ.cvar (CBinding.inst C)) := by
   constructor
@@ -756,12 +794,29 @@ def CVarSubst.instantiate {Γ : Context n m k} :
     cases hb
     simp [SType.crename_id]
     constructor; trivial
-
--- structure OmniMap (n m k n' m' k' : Nat) where
---   map : FinFun n n'
---   tmap : FinFun m m'
---   cmap : FinFun k k'
-
--- structure OmniSubst (Γ : Context n m k) (f : OmniMap n m k n' m' k') (Δ : Context n' m' k') where
+  case cmap_bound =>
+    intro c b0 hb
+    have h := Context.cvar_cbound_inv hb
+    cases h
+    case inl h =>
+      have ⟨he1, he2⟩ := h
+      subst he1
+      cases b0 <;> cases he2
+      constructor
+    case inr h =>
+      have ⟨b1, c1, hb1, he1, he2⟩ := h
+      cases he2
+      cases b1 <;> cases he1
+      rename_i cb
+      simp [FinFun.id, CBound.crename_id]
+      cases cb
+      case star => constructor
+      case upper D0 =>
+        constructor
+        apply Subcapt.cbound
+        rw [<- CaptureSet.cweaken_def]
+        rw [<- CBound.cweaken_upper]
+        rw [<- CBinding.cweaken_bound]
+        constructor; easy
 
 end Capless
